Refactoring (#1730)
The goal of this refactor is to support:

- keeping around more than one definition of low-equivalence / low-projection
and some of the lower-level theorems about those (though they might not
really be hot-swappable in the top-level proofs since some properties will be
available with one set of definitions but not in the other)
- having multiple runtime models that can benefit from some common definitions
- having multiple security properties and disconnecting the property
definitions from the models that have them.

experimental/ni_coq/vfiles/LowEquivalences.v
@@ -6,9 +6,9 @@ From OakIFC Require Import
     Parameters
     GenericMap
     Lattice
+    State
     Events
-    RuntimeModel
-    EvAugSemantics.
+    ModelTypes.
 
 From RecordUpdate Require Import RecordSet.
 Import RecordSetNotations.
@@ -139,7 +139,7 @@ Definition state_low_eq := fun ell s1 s2 =>
     and discussion in PossibilisticNI.v
 *)
 
-Inductive trace_low_eq: level -> trace -> trace -> Prop :=
+Inductive trace_low_eq: @trace_low_eqT (state * (@labeled event)) :=
     | NilEQ ell: trace_low_eq ell [] []
     | AddBoth ell xs xe ys ye t1 t2:
         trace_low_eq ell t1 t2 ->
