experimental/ni_coq/vfiles/ModelTypes.v
@@ -1,0 +1,15 @@
+Require Import List.
+From OakIFC Require Import
+    Parameters
+    Lattice.
+
+Definition trace {TraceEltT: Type} := @list TraceEltT.
+Definition trace_semanticsT {TraceEltT: Type} :=
+    (@trace TraceEltT) -> (@trace TraceEltT) -> Prop.
+
+Definition trace_low_eqT {TraceEltT: Type} :=
+    level -> (@trace TraceEltT) -> (@trace TraceEltT) -> Prop.
+
+Definition low_proj_t {A: Type}: Type := level -> A -> A.
+
+Definition low_eq_t {A: Type}: Type := level -> A -> A -> Prop.
