experimental/ni_coq/vfiles/Unwind.v
@@ -4,12 +4,12 @@ From OakIFC Require Import
     Lattice
     Parameters
     GenericMap
-    RuntimeModel
-    EvAugSemantics
+    State
     Events
+    ModelSemUtils
     LowEquivalences
-    Tactics
-    NIUtilTheorems.
+    NIUtilTheorems
+    Tactics.
 From RecordUpdate Require Import RecordSet.
 Import RecordSetNotations.
 Local Open Scope map_scope.
@@ -39,11 +39,11 @@ Proof.
     destruct s1, s2; intros *.
     inversion 1; subst.
     cbv [state_upd_node state_low_eq state_low_proj set] in *.
-    cbn [RuntimeModel.nodes RuntimeModel.chans] in *.
+    cbn [State.nodes State.chans] in *.
     split; try congruence; intros.
     destruct (dec_eq_nid id nid).
     - rewrite e in *. specialize (H0 nid).
-    cbv [node_state_low_proj low_proj fnd RuntimeModel.lbl RuntimeModel.obj] in *.
+    cbv [node_state_low_proj low_proj fnd State.lbl State.obj] in *.
     simpl in *. erewrite upd_eq. erewrite upd_eq.
     destruct (nodes nid), (nodes0 nid).
     pose proof (top_is_top ell).
@@ -55,8 +55,8 @@ Proof.
     pose proof (ord_anti ell top ltac:(eauto) ltac:(eauto));
     congruence.
     - specialize (H0 nid).
-    cbv [node_state_low_proj low_proj fnd RuntimeModel.lbl 
-        RuntimeModel.obj] in *.
+    cbv [node_state_low_proj low_proj fnd State.lbl 
+        State.obj] in *.
     simpl in *. erewrite upd_neq; auto. erewrite upd_neq; auto.
 Qed.
 
@@ -106,6 +106,19 @@ Proof.
     unfold s_set_call.
     destruct (s1.(nodes).[? id]) eqn:E1; destruct (s2.(nodes).[? id]) eqn:E2.
 Admitted.
+
+Hint Resolve state_upd_chan_unwind chan_append_unwind chan_low_proj_loweq
+    chan_low_proj_idempotent state_upd_node_unwind set_call_unwind
+    state_upd_chan_unwind state_low_proj_loweq state_upd_chan_labeled_unwind
+    state_upd_node_labeled_unwind state_chan_append_labeled_unwind
+    labeled_low_proj_loweq: unwind.
+Hint Extern 4 (node_low_eq _ _ _) => reflexivity : unwind.
+Hint Extern 4 (chan_low_eq _ _ _) => reflexivity : unwind.
+(* meant to be case where we have (cleq ch (proj ch) ) and want to swap order *)
+Hint Extern 4 (chan_low_eq _ _ (chan_low_proj _ _)) => symmetry : unwind.
+Hint Extern 4 (state_low_eq _ _ (state_low_proj _ _)) => symmetry : unwind.
+Hint Extern 2 (chan_low_proj _ _ = chan_low_proj _ _)
+=> simple eapply chan_low_proj_loweq : unwind.
 
 Hint Resolve state_upd_chan_unwind chan_append_unwind
                 set_call_unwind state_upd_node_unwind
